src/MerkleTree.New.High.Correct.Insertion.fsti
@@ -1,0 +1,41 @@
+module MerkleTree.New.High.Correct.Insertion
+
+
+open FStar.Classical
+open FStar.Ghost
+open FStar.Seq
+
+module S = FStar.Seq
+
+module MTS = MerkleTree.Spec
+open MerkleTree.New.High
+open MerkleTree.New.High.Correct.Base
+
+/// Correctness of insertion
+
+val mt_insert_inv_preserved:
+  #hsz:pos ->
+  mt:merkle_tree #hsz {mt_wf_elts mt /\ mt_not_full mt} -> v:hash ->
+  olds:hashess #hsz {S.length olds = 32 /\ mt_olds_inv #hsz 0 (MT?.i mt) olds} ->
+  Lemma (requires (mt_inv #hsz mt olds))
+        (ensures (mt_inv #hsz (mt_insert mt v) olds))
+
+/// Correctness of `create_mt`
+
+val empty_olds_inv:
+  #hsz:pos -> #f:MTS.hash_fun_t #hsz ->
+  lv:nat{lv <= 32} ->
+  Lemma (requires True)
+        (ensures (mt_olds_inv #hsz lv 0 (empty_hashes 32)))
+
+val create_empty_mt_inv_ok:
+  #hsz:pos -> #f:MTS.hash_fun_t #hsz ->
+  unit ->
+  Lemma (empty_olds_inv #_ #f 0;
+        mt_inv #hsz (create_empty_mt #_ #f ()) (empty_hashes 32))
+
+val create_mt_inv_ok:
+  #hsz:pos -> #f:MTS.hash_fun_t #hsz ->
+  init:hash ->
+  Lemma (empty_olds_inv #_ #f 0;
+        mt_inv #hsz (mt_create hsz f init) (empty_hashes 32))
