src/MerkleTree.New.High.Correct.Path.fst
@@ -27,14 +27,6 @@ open MerkleTree.New.High
 
 /// Correctness of path generation
 
-val path_spec:
-  #hsz:pos ->
-  k:nat ->
-  j:nat{k <= j} ->
-  actd:bool ->
-  p:path #hsz {S.length p = mt_path_length k j actd} ->
-  GTot (sp:S.seq (MTS.padded_hash #hsz){S.length sp = log2c j})
-       (decreases j)
 let rec path_spec #hsz k j actd p =
   if j = 0 then S.empty
   else (if k % 2 = 0
@@ -275,21 +267,6 @@ let mt_get_path_inv_ok_ #_ #f lv i j olds hs rhs k p acc actd =
     k acc actd
 #pop-options
 
-val mt_get_path_inv_ok:
-  #hsz:pos -> 
-  mt:merkle_tree #hsz {mt_wf_elts mt} ->
-  olds:hashess #hsz {S.length olds = 32 /\ mt_olds_inv #hsz 0 (MT?.i mt) olds} ->
-  idx:nat{MT?.i mt <= idx && idx < MT?.j mt} ->
-  drt:hash ->
-  Lemma (requires (MT?.j mt > 0 /\ mt_inv mt olds))
-        (ensures (let j, p, rt = mt_get_path mt idx drt in
-                 j == MT?.j mt /\
-                 mt_root_inv #_ #(MT?.hash_fun mt) (mt_base mt olds) hash_init false rt /\
-                 S.head p == S.index (mt_base mt olds) idx /\
-                 (assert (S.length (S.tail p) == mt_path_length idx (MT?.j mt) false);
-                 S.equal (path_spec idx (MT?.j mt) false (S.tail p))
-                         (MTS.mt_get_path #_ #(MT?.hash_fun mt) #(log2c j) (mt_spec mt olds) idx))))
-
 (* This proof is not that difficult to Z3, but it sometimes triggers
 an internal overflow in Z3. So, restart the solver and use a retry 2 to
 work around it in most cases. *)
@@ -397,14 +374,5 @@ let rec mt_verify_ok_ #hsz #f k j p ppos acc actd =
   end
 #pop-options
 
-val mt_verify_ok:
-  #hsz:pos -> #f:MTS.hash_fun_t ->
-  k:nat ->
-  j:nat{k < j} ->
-  p:path #hsz {S.length p = 1 + mt_path_length k j false} ->
-  rt:hash #hsz ->
-  Lemma (mt_verify #_ #f k j p rt <==>
-        MTS.mt_verify #_ #f #(log2c j)
-          (path_spec k j false (S.tail p)) k (MTS.HRaw (S.head p)) (MTS.HRaw rt))
 let mt_verify_ok #_ #f k j p rt =
   mt_verify_ok_ #_ #f k j p 1 (S.head p) false
