src/MerkleTree.New.High.Correct.Rhs.fsti
@@ -1,0 +1,25 @@
+module MerkleTree.New.High.Correct.Rhs
+
+open FStar.Ghost
+
+module S = FStar.Seq
+
+open MerkleTree.New.High
+open MerkleTree.New.High.Correct.Base
+
+/// Correctness of rightmost hashes
+
+val mt_get_root_inv_ok:
+  #hsz:pos ->
+  mt:merkle_tree #hsz {mt_wf_elts mt} -> drt:hash ->
+  olds:hashess #hsz {S.length olds = 32 /\ mt_olds_inv #hsz 0 (MT?.i mt) olds} ->
+  Lemma (requires (mt_inv mt olds))
+        (ensures (let nmt, rt = mt_get_root mt drt in
+                 // Only `MT?.rhs` and `MT?.mroot` are changed.
+                 MT?.i mt == MT?.i nmt /\
+                 MT?.j mt == MT?.j nmt /\
+                 MT?.hs mt == MT?.hs nmt /\
+                 // A Merkle tree with new `MT?.rhs` and `MT?.mroot` is valid.
+                 mt_inv nmt olds /\
+                 // A returned root is indeed the Merkle root.
+                 rt == MT?.mroot nmt))
